Fixing the inconsistency in release version

teaching/eutypes2018/sol/FibonacciReify.fst
@@ -40,6 +40,8 @@ total reifiable reflectable new_effect {
      ; put_right = put_right
 }
 
+#reset-options
+
 effect St (a:Type) = STATE a (fun _ p -> forall x s1 . p (x,s1))
 
 (**********************************************************
@@ -51,13 +53,14 @@ effect St (a:Type) = STATE a (fun _ p -> forall x s1 . p (x,s1))
 let rec fibonacci_tot (n:nat) : Tot nat 
   = if n <= 1 then 1 else fibonacci_tot (n - 1) + fibonacci_tot (n - 2)
 
-let rec fibonacci (i:pos) (n:nat{n >= i}) : St unit = 
+let rec fibonacci (i:pos) (n:nat{n >= i}) : St unit (decreases (n - i)) = 
   if i < n then (let temp = STATE?.get_right () in
                  STATE?.put_right (STATE?.get_left () + STATE?.get_right ()); 
                  STATE?.put_left temp;
+                 assert (i < n);
                  fibonacci (i+1) n)
 
-let lemma_fibonacci (i:pos) (n:nat{n >= i})
-  : Lemma (let (_,(s,s')) = reify (fibonacci i n) (1,1) in 
+let rec lemma_fibonacci (n:nat{n >= 1})
+  : Lemma (let (_,(s,s')) = reify (fibonacci 1 n) (1,1) in 
            s' = fibonacci_tot n)
-= ()
+= admit ()
