teaching/eutypes2018/ex/SumReify.fst
@@ -32,6 +32,8 @@ total reifiable reflectable new_effect {
      ; put      = put
 }
 
+#reset-options
+
 effect St (a:Type) = STATE a (fun _ p -> forall x s1 . p (x,s1))
 
 (**********************************************************
